src/Helpers/Maps.v
@@ -1,7 +1,6 @@
 Require Import List.
 Require Import Ordering.
 Require Import ProofIrrelevance.
-Require Import Helpers.
 
 Set Implicit Arguments.
 
@@ -1471,13 +1470,3 @@ Module FMap.
   End MapKeys.
 
 End FMap.
-
-
-Instance cmp_equal_dec : forall {T} {_ : Ordering T}, EqualDec T.
-Proof.
-  unfold EqualDec; intros.
-  destruct (cmp x y) eqn:He.
-  eapply cmp_eq1 in He; eauto.
-  eapply FMap.cmp_lt_neq2 in He; eauto.
-  eapply FMap.cmp_lt_neq1 in He; eauto.
-Defined.
