src/Helpers/ProofAutomation.v
@@ -1,0 +1,15 @@
+(** * Proof automation.
+
+    To help prove various theorems, we provide some basic automation.
+    This automation takes the form of Ltac scripts that are designed
+    to solve certain types of goals, or simplify the goal in some way.
+    We also use hints (using various [Hint] statements), which is a
+    way to tell Coq which theorems should be used by tactics like
+    [auto], [eauto], [autorewrite], and so on.
+  *)
+
+Require Export Helpers.ProofAutomation.Abstract.
+Require Export Helpers.ProofAutomation.ExistentialVariants.
+Require Export Helpers.ProofAutomation.Misc.
+Require Export Helpers.ProofAutomation.Propositional.
+Require Export Helpers.ProofAutomation.SimplMatch.
