src/Helpers/ProofAutomation/ExistentialVariants.v
@@ -1,0 +1,34 @@
+(** * Additional support for evar-creating versions of tactics *)
+
+(* safe version of repeat eexists (which will unfold definitions) *)
+Ltac descend :=
+  repeat match goal with
+         | |- exists _, _ => eexists
+         end.
+
+Ltac especialize H :=
+  match type of H with
+  | forall (x:?T), _ =>
+    let x := fresh x in
+    evar (x:T);
+    specialize (H x);
+    subst x
+  end.
+
+Local Ltac _especialize H :=
+  lazymatch type of H with
+  | forall (x:?T), _ => let x := fresh x in
+                  lazymatch type of T with
+                  | Prop => unshelve (evar (x:T);
+                        specialize (H x);
+                        subst x)
+                  | _ => evar (x:T);
+                        specialize (H x);
+                        subst x
+                  end
+  end.
+
+Ltac epose_proof H :=
+  let H' := fresh in
+  pose proof H as H';
+  repeat (_especialize H').
