src/Helpers/ProofAutomation/Misc.v
@@ -1,0 +1,37 @@
+Require Import Arith.
+Require Import Bool.
+Require Import List.
+Require Import String.
+Require Import Eqdep.
+
+Require Import ProofAutomation.Propositional.
+
+(** ** Other proof automation helpers *)
+
+Ltac sigT_eq :=
+  match goal with
+  | [ H: existT ?P ?a _ = existT ?P ?a _ |- _ ] =>
+    apply Eqdep.EqdepTheory.inj_pair2 in H; subst
+  end.
+
+Ltac inv_clear H := inversion H; clear H; subst; repeat sigT_eq.
+
+(** substitute variables that are let bindings (these can be created with [set
+(x:=value)] and appear in the context as [v := def]) *)
+Ltac subst_var :=
+  repeat match goal with
+  | [ v := _ |- _ ] => subst v
+  end.
+
+Create HintDb false.
+
+Ltac solve_false :=
+  solve [ exfalso; eauto with false ].
+
+Ltac rename_by_type type name :=
+  match goal with | x : type |- _ => rename x into name end.
+
+Ltac induct H :=
+  induction H; repeat sigT_eq; propositional.
+Ltac invert H :=
+  inversion H; repeat sigT_eq; propositional; repeat sigT_eq.
