src/Spec/CompileLoop.v
@@ -1,6 +1,6 @@
 Require Import ConcurExec.
 Require Import Equiv ProcMatch.
-Require Import Helpers.Helpers.
+Require Import ProofAutomation.
 Require Import FunctionalExtensionality.
 Require Import Omega.
 Require Import List.
