src/Spec/Trace.v
@@ -1,4 +1,4 @@
-Require Import Helpers.Helpers.
+Require Import ProofAutomation.
 
 Require List.
 Import List.ListNotations.
